theories/security.v
@@ -13,6 +13,7 @@ Require Import semantics.
 Require Import trace.
 Require Import types.
 Require Import util.
+Require Import termination.
 
 Section SecurityMain.
 
@@ -454,6 +455,7 @@ Lemma do_eval_udf_ok: ∀ args_types ret op f β tr tp gb args policy trace res,
   do_eval_udf args_types ret op f (β, tr, tp, gb) args (Some (policy, trace, res)) →
   Forall (λ x, label_transition_valid x) trace ∧ branch_ok policy trace.
 Proof.
+  
 Admitted.
 
 Lemma eval_udf_ok: ∀ arg_types ret op f args β β' tr tr' tp tp' gb gb' v,
