theories/termination.v
@@ -1,0 +1,454 @@
+Require Import Arith.
+Require Import Arith.Compare.
+Require Import Lia.
+Require Import List.
+Require Import ListSet.
+Require Import Logic.Eqdep_dec Logic.EqdepFacts.
+Require Import String.
+Require Import Unicode.Utf8.
+
+Require Import config.
+Require Import data_model.
+Require Import expression.
+Require Import trace.
+Require Import types.
+Require Import lattice.
+Require Import ordering.
+Require Import relation.
+Require Import util.
+Require Import semantics.
+
+Lemma join_policy_and_trace_terminate: ∀ l1 l2 com tr1 tr2, ∃ res,
+  join_policy_and_trace l1 l2 com tr1 tr2 res.
+Proof.
+  induction l1; destruct l2; destruct com; intros.
+  1-7: exists (Some (tr1 ⊍ tr2)); constructor; auto.
+  all: remember a as hd1. remember n as hd2.
+    destruct (label_lookup tr1 hd1) eqn: Hhd1, (label_lookup tr2 hd2) eqn: Hhd2.
+    2-4: exists None; eapply join_policy_and_trace_lookup_err; eauto.
+    all: assert (tr1 ≠ nil ∧ tr2 ≠ nil) as Hpreq.
+    {
+      destruct tr1; destruct tr2; try discriminate.
+      split; discriminate. 
+    }
+    destruct Hpreq.
+    destruct tr1; destruct tr2; try discriminate.
+    destruct (IHl1 l2 com tr1 tr2).
+    destruct x as [tr|].
+    - pose (extract_policy t) as p1.
+      pose (extract_policy t0) as p2.
+      destruct (Policy.policy_join_terminate p1 p2) as [pjoin].
+      exists (Some ((n0, (TrBranch prov_join pjoin (t :: t0 :: nil))) :: tr)).
+      eapply join_policy_and_trace_cons_ok; eauto.
+    - exists None. eapply join_policy_and_trace_cons_err; eauto.
+Qed.
+
+Lemma relation_join_by_prv_helper_terminate: ∀ s1 s2 join_by t r ε1 ε2 p1 p2,
+  ∃ res, relation_join_by_prv_helper s1 s2 join_by t r ε1 ε2 p1 p2 res.
+Proof.
+  induction r; intros.
+  - subst. exists (Some (nil, calculate_budget ε1 ε2, (p1 ⊍ p2))). constructor; auto.
+  - rename t into t1. rename a into t2.
+    destruct (tuple_concat_by s1 s2 join_by t1 t2) as [ [t' [ [ index_lhs index_rhs ] comid ] ]|] eqn: H1.
+    + destruct (join_policy_and_trace_terminate index_lhs index_rhs comid p1 p2). destruct x as [tr_merged|] eqn: H2.
+      * destruct (IHr ε1 ε2 p1 p2). destruct x0 as [ [ [r_cons ε_cons] tr_cons] |].
+        -- exists (Some (t' :: r_cons, calculate_budget (calculate_budget ε1 ε2) ε_cons, (tr_merged ⊍ tr_cons))).
+           eapply E_JoinConsOk; intuition; try discriminate; eauto.
+        -- exists None. eapply E_JoinConsError3; intuition; try discriminate; eauto.
+      * exists None. eapply E_JoinConsError2; intuition; try discriminate; eauto.
+    + exists None. eapply E_JoinConsError1; intuition; try discriminate; eauto.
+Qed.
+
+Lemma relation_join_by_prv_terminate: ∀ s1 s2 join_by r1 r2 ε1 ε2 p1 p2, ∃ res,
+  relation_join_by_prv s1 s2 join_by r1 r2 ε1 ε2 p1 p2 res.
+Proof.
+  intros. destruct s1; destruct s2.
+  - exists (Some (nil, O, nil)). constructor; intuition.
+  - exists (Some (nil, O, nil)). constructor; intuition.
+  - exists (Some (nil, O, nil)). constructor; intuition.
+  - induction r1; destruct r2.
+    + exists (Some (nil, O, nil)). apply E_RelationJoinNil. intuition.
+    + exists (Some (nil, O, nil)). apply E_RelationJoinNil. intuition.
+    + exists (Some (nil, O, nil)). apply E_RelationJoinNil. intuition.
+    + destruct (relation_join_by_prv_helper_terminate
+                  (a :: s1) (a0 :: s2) join_by a1 (t :: r2) ε1 ε2 p1 p2).
+      destruct IHr1.
+      destruct x; destruct x0.
+      * destruct p as[ [ r_hd β_hd ] p_hd ].
+        destruct p0 as[ [ r_cons β_cons ] p_cons ].
+        pose (merge_env p_hd p_cons) as p_out.
+        pose (calculate_budget β_hd β_cons) as β_out.
+        exists (Some (r_hd ++ r_cons, β_out, p_out)).
+        eapply E_RelationJoinConsOk; intuition; try discriminate; eauto.
+      * exists None. destruct p as[ [ r_hd β_hd ] p_hd ].
+        eapply E_RelationJoinConsErr; intuition; try discriminate; eauto.
+      * exists None. econstructor; intuition; try discriminate; auto.
+      * exists None. econstructor; intuition; try discriminate; auto.
+Qed.
+
+Lemma relation_join_by_prv_deterministic: ∀ s1 s2 join_by r1 r2 ε1 ε2 p1 p2 res1 res2,
+  relation_join_by_prv s1 s2 join_by r1 r2 ε1 ε2 p1 p2 res1 →
+  relation_join_by_prv s1 s2 join_by r1 r2 ε1 ε2 p1 p2 res2 →
+  res1 = res2.
+Proof.
+Admitted.
+
+Theorem eval_terminate: ∀ e b β tp proxy, ∃ env, eval 100 e b (β, tp, proxy) env.
+Proof.
+  induction e; intros.
+  - 
+Admitted.
+
+Theorem eval_expr_terminate: ∀ b β tr tp proxy e, ∃ res, eval_expr b (β, tr) tp proxy e res.
+Proof.
+  intros.
+  destruct (eval_terminate e b (β, tr) tp proxy) as [env].
+  exists env.
+  constructor. assumption.
+Qed.
+
+Theorem eval_predicate_in_relation_terminate:
+  ∀ s r β tr e, ∃ res, eval_predicate_in_relation s r β tr e res.
+Proof.
+  induction r; intros.
+  - exists (Some (nil, β, tr)). constructor. reflexivity.
+  - 
+Admitted.
+
+Theorem eval_aggregate_terminate:
+  ∀ s s_agg gb b agg expr β tr r, ∃ res, eval_aggregate s s_agg gb b agg expr β tr r res.
+Proof.
+Admitted.
+
+
+Theorem apply_proj_in_relation_deterministic: ∀ s s' r pl β tr res1 res2,
+  apply_proj_in_relation s s' r pl β tr res1 →
+  apply_proj_in_relation s s' r pl β tr res2 →
+  res1 = res2.
+Proof. Admitted.
+
+Theorem apply_proj_in_relation_terminate: ∀ s s' r pl β tr,
+  ∃ res, apply_proj_in_relation s s' r pl β tr res.
+Proof. Admitted.
+
+Theorem operator_deterministic: ∀ db o c1 c2, 
+  ⟦ db o ⟧ ⇓ ⟦ c1 ⟧ →
+  ⟦ db o ⟧ ⇓ ⟦ c2 ⟧ →
+  c1 = c2.
+Proof.
+  induction o; intros.
+  - inversion H0; inversion H; subst; auto; try discriminate.
+  - inversion H0; inversion H; subst; auto; try discriminate;
+    try (rewrite H5 in H12; inversion H12); auto; 
+    try (rewrite H4 in H11; inversion H11; subst); auto.
+    try (rewrite H4 in H10; inversion H10; subst); auto.
+    + contradiction.
+    + contradiction.
+    + rewrite H4 in H10. discriminate.
+  - destruct c1; destruct c2.
+    + reflexivity.
+    (* + inversion H0; subst; try discriminate.
+    + inversion H; subst; try discriminate.
+      * inversion H0; subst; try discriminate.
+      * destruct H7; subst.
+        -- inversion H0; subst.
+           specialize IHo1 with (c1 := (ConfigOut (RelationWrapped s r') (⟨ db' β' tr' ⟩))) (c2 := ConfigError).
+           apply IHo1 in H9.
+           ++ discriminate.
+           ++ assumption.
+        -- inversion H0; subst.
+           specialize IHo2 with (c1 := ConfigError) (c2 := (ConfigOut (RelationWrapped s r'') (⟨ db'' Γ'' β'' p'' ⟩))).
+           apply IHo2 in H11.
+           ++ discriminate.
+           ++ assumption.
+      * inversion H0; subst; try discriminate.
+        inversion H8. subst.
+        (* The contradiction occurs when s1 ≠ s2 where s = s1 ∧ s = s2. *)
+        specialize IHo1 with (c1 := (ConfigOut (RelationWrapped s1 r') (⟨ db' β' tr' ⟩)))
+                             (c2 := (ConfigOut (RelationWrapped s r'0) (⟨ db'0 Γ'0 β'0 p'0 ⟩))).
+        specialize IHo2 with (c1 := (ConfigOut (RelationWrapped s2 r'') (⟨ db'' Γ'' β'' p'' ⟩)))
+                             (c2 := (ConfigOut (RelationWrapped s r''0) (⟨ db''0 Γ''0 β''0 p''0 ⟩))).
+        apply IHo2 in H7. inversion H7. subst.
+        apply IHo1 in H5. inversion H5. subst.
+        -- exfalso. apply H9. reflexivity.
+        -- assumption.
+        -- assumption.
+    + inversion H; subst; try discriminate.
+    + inversion H0; subst; try discriminate.
+    + inversion H; subst; try discriminate.
+    + inversion H0; subst; try discriminate.
+      * inversion H; subst; try discriminate.
+      * destruct H7; subst.
+        -- inversion H; subst; try discriminate.
+           specialize IHo1 with (c1 := (ConfigOut (RelationWrapped s r') (⟨ db' β' tr' ⟩))) (c2 := ConfigError).
+           apply IHo1 in H9.
+           ++ discriminate.
+           ++ assumption.
+        -- inversion H; subst.
+           specialize IHo2 with (c1 := ConfigError) (c2 := (ConfigOut (RelationWrapped s r'') (⟨ db'' Γ'' β'' p'' ⟩))).
+           apply IHo2 in H11.
+           ++ discriminate.
+           ++ assumption.
+      * inversion H; subst; try discriminate.
+        inversion H8. subst.
+        (* The contradiction occurs when s1 ≠ s2 where s = s1 ∧ s = s2. *)
+        specialize IHo1 with (c1 := (ConfigOut (RelationWrapped s1 r') (⟨ db' β' tr' ⟩)))
+                             (c2 := (ConfigOut (RelationWrapped s r'0) (⟨ db'0 Γ'0 β'0 p'0 ⟩))).
+        specialize IHo2 with (c1 := (ConfigOut (RelationWrapped s2 r'') (⟨ db'' Γ'' β'' p'' ⟩)))
+                             (c2 := (ConfigOut (RelationWrapped s r''0) (⟨ db''0 Γ''0 β''0 p''0 ⟩))).
+        apply IHo2 in H7. inversion H7. subst.
+        apply IHo1 in H5. inversion H5. subst.
+        -- exfalso. apply H9. reflexivity.
+        -- assumption.
+        -- assumption.
+    + inversion H0; subst; try discriminate.
+    + inversion H; inversion H0; subst; try discriminate.
+      * inversion H8. subst. inversion H4. subst. assumption.
+      * inversion H16. subst.
+        specialize IHo2 with (c1 := (ConfigOut (RelationWrapped s0 r''0) (⟨ db''0 Γ''0 β''0 p''0 ⟩)))
+                             (c2 := (ConfigOut (RelationWrapped s r'') (⟨ db'' Γ'' β'' p'' ⟩))).
+        specialize IHo1 with (c1 := (ConfigOut (RelationWrapped s0 r'0) (⟨ db'0 Γ'0 β'0 p'0 ⟩)))
+                             (c2 := (ConfigOut (RelationWrapped s r') (⟨ db' β' tr' ⟩))).
+        intuition. inversion H3. inversion H1. subst.
+        (*
+          Now we have some weird equality over dependent types:
+                    existT P p a = existT P p b
+                    ^^^^^: ∀ [A : Type] (P : A → Type) (x : A), P x → {x : A & P x}
+        
+           The reason for that is that the index `s` appears on the types of `a`
+           and `b` cannot be generalized when typing the equality `a = b` which
+           is required for `inversion` tactic.
+           
+           `existT` is the constructor for the dependent pair type, which "hides"
+           the index and allows Coq to avoid this problem in the general case,
+           producing a statement which is slightly similar.
+
+           `inj_pair2_eq_dec` is a lemma that allows us to `inversion` equality of
+            dependent pairs given that the index is decidable.
+         *)
+
+        apply inj_pair2_eq_dec in H5, H13; subst; try reflexivity;
+        apply list_eq_dec; apply attribute_eq_dec.
+  - inversion H0; inversion H; subst; try discriminate; auto.
+    + intuition; subst.
+      * apply (IHo1 ConfigError) in H13. discriminate. assumption.
+      * apply (IHo2 ConfigError) in H15. discriminate. assumption.
+    + inversion H14. subst. clear H14.
+      apply (IHo1 (ConfigOut (RelationWrapped s1 r') (⟨ db' β' tr' ⟩))) in H15.
+      apply (IHo2 (ConfigOut (RelationWrapped s2 r'') (⟨ db'' Γ'' β'' p'' ⟩))) in H17.
+      inversion H15. inversion H17. subst.
+      apply inj_pair2_eq_dec in H3, H12; subst. 
+      * eapply relation_join_by_prv_deterministic with (res2 := None) in H20.
+        inversion H20. assumption.
+      * apply list_eq_dec; apply attribute_eq_dec.
+      * apply list_eq_dec; apply attribute_eq_dec.
+      * assumption.
+      * assumption.
+    + intuition; inversion H15; subst.
+      * apply (IHo1 ConfigError) in H5. discriminate. assumption.
+      * apply (IHo2 ConfigError) in H7. discriminate. assumption.
+    + inversion H15. subst. clear H15.
+      apply (IHo1 (ConfigOut (RelationWrapped s1 r') (⟨ db' β' tr' ⟩))) in H16.
+      apply (IHo2 (ConfigOut (RelationWrapped s2 r'') (⟨ db'' Γ'' β'' p'' ⟩))) in H18.
+      inversion H16. inversion H18. subst.
+      apply inj_pair2_eq_dec in H3, H12; subst. 
+      * eapply relation_join_by_prv_deterministic with (res2 := None) in H10.
+        inversion H10. assumption.
+      * apply list_eq_dec; apply attribute_eq_dec.
+      * apply list_eq_dec; apply attribute_eq_dec.
+      * assumption.
+      * assumption.
+    + apply (IHo1 (ConfigOut (RelationWrapped s1 r') (⟨ db' β' tr' ⟩))) in H16.
+      apply (IHo2 (ConfigOut (RelationWrapped s2 r'') (⟨ db'' Γ'' β'' p'' ⟩))) in H18.
+      inversion H15. inversion H18. inversion H16. subst.
+      apply inj_pair2_eq_dec in H9, H19. subst.
+      eapply relation_join_by_prv_deterministic with (res2 := (Some (rout, Γout, βout, pout))) in H21.
+      * inversion H21. subst. reflexivity.
+      * assumption.
+      * apply list_eq_dec; apply attribute_eq_dec.
+      * apply list_eq_dec; apply attribute_eq_dec.
+      * assumption.
+      * assumption.
+  - inversion H0; inversion H; subst; intuition; auto; subst; try discriminate.
+    + apply IHo with (c1 := ConfigOut (RelationWrapped s nil) (⟨ db' β' tr' ⟩)) in H13.
+      inversion H12. subst. inversion H13. subst. apply inj_pair2_eq_dec in H6. subst.
+      * exfalso. apply H2. auto.
+      * apply list_eq_dec; apply attribute_eq_dec.
+      * assumption.
+    + apply IHo with (c1 := (ConfigOut (RelationWrapped nil r) (⟨ db' β' tr' ⟩))) in H13.
+      inversion H12. subst. inversion H13. subst. apply inj_pair2_eq_dec in H6. subst.
+      * exfalso. apply H1. auto.
+      * apply list_eq_dec; apply attribute_eq_dec.
+      * assumption.
+    + apply IHo with (c1 := (ConfigOut (RelationWrapped s nil) (⟨ db' β' tr' ⟩))) in H13.
+      inversion H12. subst. inversion H13. subst. apply inj_pair2_eq_dec in H6. subst.
+      * exfalso. apply H2. auto.
+      * apply list_eq_dec; apply attribute_eq_dec.
+      * assumption.
+    + apply IHo with (c1 :=(ConfigOut (RelationWrapped nil r) (⟨ db' β' tr' ⟩))) in H13.
+      inversion H12. subst. inversion H13. subst. apply inj_pair2_eq_dec in H6. subst.
+      * exfalso. apply H1. auto.
+      * apply list_eq_dec; apply attribute_eq_dec.
+      * assumption.
+    + apply IHo with (c1 := (ConfigOut (RelationWrapped s nil) (⟨ db' β' tr' ⟩))) in H13.
+      inversion H12. subst. inversion H13. subst. apply inj_pair2_eq_dec in H6. subst.
+      * exfalso. apply H2. auto.
+      * apply list_eq_dec; apply attribute_eq_dec.
+      * assumption.
+    + apply IHo with (c1 :=(ConfigOut (RelationWrapped nil r) (⟨ db' β' tr' ⟩))) in H13.
+      inversion H12. subst. inversion H13. subst. apply inj_pair2_eq_dec in H6. subst.
+      * exfalso. apply H1. auto.
+      * apply list_eq_dec; apply attribute_eq_dec.
+      * assumption.
+    + apply IHo with (c1 := (ConfigOut (RelationWrapped s' r') (⟨ db' β' tr' ⟩))) in H17.
+      inversion H16. subst. inversion H17. subst. apply inj_pair2_eq_dec in H6. subst.
+      * exfalso. apply H2. auto.
+      * apply list_eq_dec; apply attribute_eq_dec.
+      * assumption.
+    + apply IHo with (c1 :=(ConfigOut (RelationWrapped s' r') (⟨ db' β' tr' ⟩))) in H17.
+      inversion H16. subst. inversion H17. subst. apply inj_pair2_eq_dec in H6. subst.
+      * exfalso. apply H1. auto.
+      * apply list_eq_dec; apply attribute_eq_dec.
+      * assumption.
+    + apply IHo with (c1 := (ConfigOut (RelationWrapped s' r') (⟨ db' β' tr' ⟩))) in H17.
+      inversion H16. subst. inversion H17. subst. apply inj_pair2_eq_dec in H10. subst.
+      (* Subsitute pl' and pl'0. *)
+      rewrite <- H8 in H20. inversion H20. subst.
+      (* Then we are able to substite schemas. *)
+      rewrite <- H9 in H21. inversion H21. subst.
+      * specialize apply_proj_in_relation_deterministic
+          with
+          (s := s'0) (s' := s'')
+          (r := r'0) (pl := pl')
+          (Γ := Γ'0) (β := β'0) (p := p'0)
+          (res1 := Some (r'', β'', tr'')) (res2 := Some (r''0, Γ''0, β''0, p''0)).
+          intros.
+        apply H6 in H11. inversion H11. subst.
+        reflexivity. assumption.
+      * apply list_eq_dec; apply attribute_eq_dec.
+      * assumption.
+    + apply IHo with (c1 := (ConfigOut (RelationWrapped s' r') (⟨ db' β' tr' ⟩))) in H17.
+      inversion H16. subst. inversion H17. subst. apply inj_pair2_eq_dec in H10. subst.
+      rewrite <- H8 in H20. inversion H20. subst.
+      rewrite <- H9 in H22. inversion H22. subst.
+      * specialize apply_proj_in_relation_deterministic
+          with
+          (s := s'0) (s' := s'')
+          (r := r'0) (pl := pl')
+          (Γ := Γ'0) (β := β'0) (p := p'0)
+          (res1 := Some (r'', β'', tr'')) (res2 := None).
+          intros.
+        apply H6 in H11. discriminate. assumption.
+      * apply list_eq_dec; apply attribute_eq_dec.
+      * assumption.
+    + apply IHo with (c1 := (ConfigOut (RelationWrapped s' r') (⟨ db' β' tr' ⟩))) in H18.
+      inversion H18. assumption.
+    + apply IHo with (c1 := (ConfigOut (RelationWrapped s' r') (⟨ db' β' tr' ⟩))) in H17.
+      inversion H16. subst. inversion H17. subst. apply inj_pair2_eq_dec in H10. subst.
+      rewrite <- H8 in H21. inversion H21. subst. rewrite <- H9 in H22.
+      * discriminate.
+      * apply list_eq_dec; apply attribute_eq_dec.
+      * assumption.
+    + apply IHo with (c1 := (ConfigOut (RelationWrapped s' r') (⟨ db' β' tr' ⟩))) in H16.
+      inversion H16. subst. inversion H15. subst. apply inj_pair2_eq_dec in H6. subst.
+      * exfalso. apply H2. reflexivity.
+      * apply list_eq_dec; apply attribute_eq_dec.
+      * assumption.
+    + apply IHo with (c1 := (ConfigOut (RelationWrapped s' r') (⟨ db' β' tr' ⟩))) in H16.
+      inversion H16. subst. inversion H15. subst. apply inj_pair2_eq_dec in H6. subst.
+      * exfalso. apply H1. reflexivity.
+      * apply list_eq_dec; apply attribute_eq_dec.
+      * assumption.
+    + apply IHo with (c1 := (ConfigOut (RelationWrapped s' r') (⟨ db' β' tr' ⟩))) in H16.
+      inversion H16. subst. inversion H15. subst. apply inj_pair2_eq_dec in H9. subst.
+      rewrite <- H8 in H19. inversion H19. subst.
+      rewrite <- H10 in H20. inversion H20. subst.
+      * specialize apply_proj_in_relation_deterministic
+          with
+          (s := s'0) (s' := s'')
+          (r := r'0) (pl := pl')
+          (Γ := Γ'0) (β := β'0) (p := p'0)
+          (res1 := None) (res2 := (Some (r'', β'', tr''))).
+          intros.
+        apply H6 in H11. inversion H11. assumption.
+      * apply list_eq_dec; apply attribute_eq_dec.
+      * assumption.
+    + apply IHo with (c1 := ConfigError) in H11. inversion H11. assumption.
+    + apply IHo with (c1 := (ConfigOut (RelationWrapped s' r') (⟨ db' β' tr' ⟩))) in H15.
+      inversion H15. subst. inversion H14. subst. apply inj_pair2_eq_dec in H6. subst.
+      * exfalso. apply H2. reflexivity.
+      * apply list_eq_dec; apply attribute_eq_dec.
+      * assumption.
+    + apply IHo with (c1 := (ConfigOut (RelationWrapped s' r') (⟨ db' β' tr' ⟩))) in H15.
+      inversion H15. subst. inversion H14. subst. apply inj_pair2_eq_dec in H6. subst.
+      * exfalso. apply H1. reflexivity.
+      * apply list_eq_dec; apply attribute_eq_dec.
+      * assumption.
+    + apply IHo with (c1 := (ConfigOut (RelationWrapped s' r') (⟨ db' β' tr' ⟩))) in H15.
+      inversion H15. subst. inversion H14. subst. apply inj_pair2_eq_dec in H8. subst.
+      rewrite <- H9 in H18. inversion H18. subst.
+      rewrite <- H10 in H19. inversion H19.
+      * apply list_eq_dec; apply attribute_eq_dec.
+      * assumption.
+  - inversion H0; inversion H; subst; intuition; auto; subst; try discriminate. *)
+Admitted.
+
+
+Theorem operator_always_terminate: ∀ db o, ∃ c, ⟦ db o ⟧ ⇓ ⟦ c ⟧.
+Proof.
+  (* induction o; unfold not; intros; destruct c.
+  - exfalso. auto.
+  - (* Although we don't need `s`, we need to introduce this term into the context. *)
+    pose (s := @nil attribute).
+    exists (ConfigOut (RelationWrapped nil nil) (⟨ d c b p ⟩)).
+    econstructor; reflexivity.
+  - pose (s := @nil attribute). exists (ConfigOut r c).
+    eapply E_Already with (r := r) (c := (ConfigOut r c)) (c' := c). reflexivity.
+  - exfalso. auto.
+  - destruct d eqn: Hdb.
+    + exists ConfigError. eapply E_GetRelationDbEmpty with (o := OperatorRel n); reflexivity.
+    + destruct (database_get_contexts d n) as [ [ [ r' Γ' ] p' ] | ] eqn: Hget.
+      * exists (ConfigOut r' (⟨ d Γ' b p' ⟩)).
+        eapply E_GetRelation with (db := d) (o := OperatorRel n) (Γ := c) (β := b) (p := p).
+        -- red. intros. subst. inversion H0.
+        -- reflexivity.
+        -- subst. reflexivity.
+        -- eapply Hget.
+        -- reflexivity.
+      * exists ConfigError.
+        eapply E_GetRelationError with (db := d) (o := OperatorRel n) (Γ := c) (β := b) (p := p).
+        -- red. intros. subst. inversion H0.
+        -- reflexivity.
+        -- subst. reflexivity.
+        -- assumption.
+        -- reflexivity.
+  - pose (s := @nil attribute). exists (ConfigOut r c).
+    eapply E_Already with (r := r) (c := (ConfigOut r c)) (c' := c). reflexivity.
+  - contradiction.
+  - (* We now introduce the existential variables into the context. *)
+    intuition. destruct H0. destruct H1.
+    destruct x; destruct x0.
+    + exists ConfigError. econstructor; try eauto.
+    + exists ConfigError. econstructor; try eauto.
+    + exists ConfigError. econstructor; try eauto.
+    + exists ConfigError. econstructor; try eauto.
+    + inversion H0; subst; try discriminate.
+    + inversion H0; subst; try discriminate.
+    + exists ConfigError. econstructor; try eauto.
+    + inversion H1; subst; try discriminate.
+    + destruct r, r0, x, x0; subst.
+      * inversion H0; subst; try discriminate.
+      * inversion H0; subst; try discriminate.
+      * inversion H0; subst; try discriminate.
+      * inversion H1; subst; try discriminate.
+      * destruct (list_eq_dec (attribute_eq_dec) s0 s).
+        -- subst.
+          pose (merged_p := merge_env p0 p1).
+          pose (merged_Γ := merge_env c0 c1).
+          pose (merged_β := calculate_budget b0 b1).
+          exists (ConfigOut (RelationWrapped s (r ++ r0)) (⟨ d1 merged_Γ merged_β merged_p ⟩)).
+          econstructor; try reflexivity; eauto.
+        -- exists ConfigError. eapply E_UnionSchemaError with (s1 := s) (s2 := s0); try eauto.
+      * (* There should be no rule for constructing nested output. *)
+        inversion H1; subst; try discriminate. *)
+Admitted.
