README.md
@@ -2,26 +2,12 @@
 
 This repository contains formalization for the dataframe data model and relational algebra semantics that captures the privacy policy and mechanically checked proofs of the correctness.
 
-## Prerequisites
+## Codebase layout
 
-You should install Coq >= 8.18.0 to ensure that this project compiles.
+We provide a quick introduction on how this Coq codebase relates to the on-paper formalism.
 
-## Compile the projects
+TODO: Make things tidier by organizing things into sub-folders.
 
-```sh
-$ cd ./theories
-$ coq_makefile -f ./_CoqProject -o Makefile
-$ make
-```
-
-Or you can use the Python script to type check the Coq project.
-
-```sh
-$ ./run
-```
-
-If the code compiles, all the proofs are successfully validated by Coq's type checker.
-
-# Note
+## Note
 
 The codebase of Picachv's Coq formalism is still untidy and will be cleaned up as soon as possible. As for now, there might some naming issues and/or inconsistent terms between the Coq code and paper descriptions. We sincerely apologize for any inconvenince and will fix it.
